src/generatedproof/controllers/deployment.v
@@ -5,6 +5,7 @@ Require Export New.generatedproof.k8s_io.api.core.v1.
 Require Export New.generatedproof.k8s_io.apimachinery.pkg.api.errors.
 Require Export New.generatedproof.k8s_io.apimachinery.pkg.apis.meta.v1.
 Require Export New.generatedproof.k8s_io.apimachinery.pkg.labels.
+Require Export New.generatedproof.k8s_io.apimachinery.pkg.types.
 Require Export New.generatedproof.k8s_io.kubernetes.pkg.controller.
 Require Export New.generatedproof.kubernetes_model.apimodel.
 Require Export New.generatedproof.reflect.
